# 2023-03-07

## Lema de Arden

Se $\varepsilon \not \in L_1$ e

$$
\begin{align*}
L &= L_1L + L_2\\
\implies L &= L_1^*L_2
\end{align*}
$$

## Exemplo

Seja a linguagem gerada pela gramática com as regras

$$
\begin{align*}
& S \to 0A | 1S | \varepsilon\\
&A \to 0S | 1A
\end{align*}
$$

Então

$$
\begin{align*}
&[S] = 0[A] + 1[S] + e\\
&[A] = 0[S] + 1[A]\\
&[A] = 1^*0[S] \quad\quad\quad\quad\quad\quad\quad\text{(Lema de Arden)}\\
&[S] = 01^*0[S] + 1[S] + e\\
&[S] = (01^*0 + 1)[S] + e\\
&[S] = (01^*0 + 1)^*
\end{align*}
$$

## Exemplo 2

$$
\begin{align*}
& S \to 0S | 1A \\
&A \to 1S | 0B | \varepsilon\\
&B \to 0A | 1B
\end{align*}
$$

Então

$$
\begin{align*}
&[S] = 0[S] + 1[A]\\
&[A] = 1[S] + 0[B] + e\\
&[B] = 0[A] + 1[B]\\\\
&[B] = 1^*0[A] \quad\quad\text{L. Arden}\\
&[A] = 1[S] + 01^*0[A] + e\\
&[A] = 01^*0[A] + (1[S] + e)\\
&[A] = (01^*0)^*(1[S]+e)\\
&[S] = 0[S] + 1(01^*0)^*(1[S]+e)\\
&[S] = (0 + 1(01^*0)^*1)[S] + 1(01^*0)^*\\
&[S] = (0 + 1(01^*0)^*1)^*1(01^*0)^*

\end{align*}
$$